Impl.Core.fsti
@@ -7,6 +7,7 @@ open Steel.Reference
 
 //module Spec = Trees
 module U = FStar.UInt64
+module M = FStar.Math.Lib
 
 #set-options "--ide_id_info_off"
 
@@ -24,9 +25,10 @@ let t (a: Type0) = ref (node a)
 // TODO: to be replaced with MAX_UINT64
 noextract
 let c = FStar.UInt.max_int 64
-let wds (a: Type0) = x:Spec.wds a{Spec.size_of_tree x <= c}
-//let tree (a: Type0) = x:Spec.tree a{fst (Spec.is_wds x)}
-//let tree (a: Type0) = Spec.tree a
+let wdm (a: Type0) = x:Spec.wdm a{
+  Spec.size_of_tree x <= c /\
+  Spec.height_of_tree x <= c
+}
 
 (**** Operations on nodes *)
 
@@ -39,7 +41,10 @@ val get_data (#a: Type0) (n: node a) : a
 inline_for_extraction noextract
 val get_size (#a: Type0) (n: node a) : ref U.t
 inline_for_extraction noextract
-val mk_node (#a: Type0) (data: a) (left right: t a) (size: ref U.t)
+val get_height (#a: Type0) (n: node a) : ref U.t
+inline_for_extraction noextract
+val mk_node (#a: Type0)
+  (data: a) (left right: t a) (size height: ref U.t)
     : Pure (node a)
       (requires True)
       (ensures (fun n ->
@@ -61,12 +66,12 @@ val is_null_t (#a: Type0) (r: t a) : (b:bool{b <==> r == null_t})
 val tree_sl (#a: Type0) (r: t a) : slprop u#1
 
 (** Selector retrieving the contents of a tree in memory *)
-val tree_sel (#a: Type0) (r: t a) : selector (wds a) (tree_sl r)
+val tree_sel (#a: Type0) (r: t a) : selector (wdm a) (tree_sl r)
 
 [@@__steel_reduce__]
 let linked_tree' (#a: Type0) (r: t a) : vprop' = {
   hp = tree_sl r;
-  t = wds a;
+  t = wdm a;
   sel = tree_sel r
 }
 
@@ -82,7 +87,7 @@ let v_linked_tree
   (h:rmem p{
     FStar.Tactics.with_tactic selector_tactic (can_be_split p (linked_tree r) /\ True)
   })
-    : GTot (wds a)
+    : GTot (wdm a)
   = h (linked_tree r)
 
 (*** Operations *)
@@ -134,17 +139,28 @@ val not_null_is_node (#opened:inames) (#a: Type0) (ptr: t a)
          Spec.Node? (v_linked_tree ptr h0) /\
          v_linked_tree ptr h0 == v_linked_tree ptr h1))
 
-val pack_tree (#opened:inames) (#a: Type0) (ptr: t a) (left right: t a) (sr: ref U.t)
+val pack_tree (#opened:inames) (#a: Type0)
+  (ptr: t a) (left right: t a) (sr hr: ref U.t)
     : SteelGhost unit
-      opened (vptr ptr `star` linked_tree left `star` linked_tree right `star` vptr sr)
+      opened
+      (vptr ptr `star`
+      linked_tree left `star`
+      linked_tree right `star`
+      vptr sr `star`
+      vptr hr)
       (fun _ -> linked_tree ptr)
       (requires (fun h0 ->
         get_left (sel ptr h0) == left /\
         get_right (sel ptr h0) == right /\
         get_size (sel ptr h0) == sr /\
+        get_height (sel ptr h0) == hr /\
         U.v (sel sr h0) == Spec.size_of_tree (v_linked_tree left h0)
-              + Spec.size_of_tree (v_linked_tree right h0)
-              + 1 /\
+                         + Spec.size_of_tree (v_linked_tree right h0)
+                         + 1 /\
+        U.v (sel hr h0) == M.max
+          (Spec.height_of_tree (v_linked_tree left h0))
+          (Spec.height_of_tree (v_linked_tree right h0))
+          + 1 /\
         U.v (sel sr h0) <= c
         ))
       (ensures (fun h0 _ h1 ->
@@ -152,8 +168,8 @@ val pack_tree (#opened:inames) (#a: Type0) (ptr: t a) (left right: t a) (sr: ref
         let l = v_linked_tree left h0 in
         let r = v_linked_tree right h0 in
         let s = sel sr h0 in
-        //let s = Spec.size_of_tree l + Spec.size_of_tree r + 1 in
-        v_linked_tree ptr h1 == Spec.Node x l r (U.v s)))
+        let h = sel hr h0 in
+        v_linked_tree ptr h1 == Spec.Node x l r (U.v s) (U.v h)))
 
 val unpack_tree (#a: Type0) (ptr: t a)
     : Steel (node a)
@@ -162,18 +178,26 @@ val unpack_tree (#a: Type0) (ptr: t a)
         vptr ptr `star`
         linked_tree (get_left node) `star`
         linked_tree (get_right node) `star`
-        vptr (get_size node))
+        vptr (get_size node) `star`
+        vptr (get_height node))
       (requires (fun h0 -> not (is_null_t ptr)))
       (ensures (fun h0 node h1 ->
         v_linked_tree ptr h0 == Spec.Node
           (get_data (sel ptr h1))
           (v_linked_tree (get_left node) h1)
           (v_linked_tree (get_right node) h1)
-          (U.v (sel (get_size node) h1)) /\
+          (U.v (sel (get_size node) h1))
+          (U.v (sel (get_height node) h1))
+        /\
         sel ptr h1 == node /\
-        U.v (sel (get_size node) h1) == Spec.size_of_tree (v_linked_tree (get_left node) h1)
-                                + Spec.size_of_tree (v_linked_tree (get_right node) h1) + 1 /\
-        U.v (sel (get_size node) h1) <= c
+        U.v (sel (get_size node) h1)
+        == Spec.size_of_tree (v_linked_tree (get_left node) h1)
+         + Spec.size_of_tree (v_linked_tree (get_right node) h1) + 1 /\
+        U.v (sel (get_height node) h1)
+        == M.max (Spec.height_of_tree (v_linked_tree (get_left node) h1))
+                 (Spec.height_of_tree (v_linked_tree (get_right node) h1)) + 1 /\
+        U.v (sel (get_size node) h1) <= c /\
+        U.v (sel (get_height node) h1) <= c
       ))
 
 (*)
